

```

import Mathlib

open Finsupp

open scoped Finset

variable {R : Type*} [CommRing R]

open MvPolynomial

/-- Lemma 2.2 :
A multivariate polynomial that vanishes on a large product finset is the zero
polynomial. -/
lemma eq_zero_of_eval_zero_at_prod_finset {σ : Type*} [Finite σ] [IsDomain R]
(P : MvPolynomial σ R) (S : σ → Finset R)
(Hdeg : ∀ i, P.degreeOf i < #(S i))
(Heval : ∀ (x : σ → R), (∀ i, x i ∈ S i) → eval x P = 0) :
P = 0 := by
  exact MvPolynomial.eq_zero_of_eval_zero_at_prod_finset P S Hdeg Heval

variable {p : ℕ} [Fact (Nat.Prime p)] {k : ℕ}

/-- Definition of elimination polynomials g_i -/
noncomputable def elimination_polynomials (A : Fin (k + 1) → Finset (ZMod p)) :
  Fin (k + 1) → MvPolynomial (Fin (k + 1)) (ZMod p) :=
  fun i => ∏ a ∈ A i, (MvPolynomial.X i - C a)

noncomputable def reduce_polynomial_degrees (P : MvPolynomial (Fin (k + 1)) (
  ZMod p))
(g : Fin (k + 1) → MvPolynomial (Fin (k + 1)) (ZMod p))
(c : Fin (k + 1) → ℕ) : MvPolynomial (Fin (k + 1)) (ZMod p) :=

P.support.sum fun m =>
  let coeff := P.coeff m
  let needs_replacement : Finset (Fin (k + 1)) :=
    Finset.filter (fun i => m i > c i) Finset.univ
  if h : needs_replacement.Nonempty then
    let i : Fin (k + 1) := needs_replacement.min' h
    let new_m : (Fin (k + 1)) →₀ ℕ :=
      Finsupp.update m i (m i - (c i + 1))
    coeff • (MvPolynomial.monomial new_m 1) * g i
  else
    coeff • MvPolynomial.monomial m 1

set_option maxHeartbeats 2000000 in
/-- **Alon-Nathanson-Ruzsa Theorem** (Theorem 2.1)
Proof strategy: Use Lemma 2.2 (eq_zero_of_eval_zero_at_prod_finset) to prove
Theorem 2.1

```

Proof outline:

1. Assume the conclusion is false, i.e., there exists a set $E \subset Z_p$ with $|E| = m$ such that restricted sumset subset E
2. Construct the polynomial $Q(x_0, \dots, x_k) = h(x_0, \dots, x_k) * \prod_{e \in E} (x_0 + \dots + x_k - e)$
 - $\deg(Q) = \deg(h) + m = \sum c_i$
 - For all $(a_0, \dots, a_k) \in \prod A_i$, we have $Q(a_0, \dots, a_k) = 0$
 - The coefficient of monomial $\prod x_i^{c_i}$ in Q is nonzero
3. For each i , define $g_i(x_i) = \prod_{a \in A_i} (x_i - a) = x_i^{c_i+1} - \sum_j b_{ij} x_i^j$
4. Construct polynomial Q_{bar} by replacing all occurrences of $x_i^{c_i+1}$ in Q with $\sum_j b_{ij} x_i^j$
 - For each $a_i \in A_i$, $g_i(a_i) = 0$, so Q_{bar} still vanishes on $\prod A_i$
 - $\deg_{\{x_i\}}(Q_{\text{bar}}) \leq c_i$
5. Apply Lemma 2.2:
 - Q_{bar} vanishes on $\prod A_i$
 - Degree in each variable $\leq c_i$
 - Therefore $Q_{\text{bar}} = 0$
6. But the coefficient of $\prod x_i^{c_i}$ in Q_{bar} is the same as in Q :
 - The replacement process doesn't affect this specific monomial
 - By assumption, this coefficient is nonzero in Q
 - Therefore it's nonzero in Q_{bar} , contradicting $Q_{\text{bar}} = 0$

Key points:

- Use polynomial replacement technique to reduce degrees to satisfy Lemma 2.2 conditions
 - The replacement process preserves the coefficient of the target monomial
 - Proof by contradiction
- /

```

theorem ANR_polynomial_method (h : MvPolynomial (Fin (k + 1)) (ZMod p))
  (A : Fin (k + 1) → Finset (ZMod p))
  (c : Fin (k + 1) → ℕ)
  (hA : ∀ i, (A i).card = c i + 1)
  (m : ℕ) (hm : m = (∑ i, c i) - h.totalDegree)
  (h_coeff : MvPolynomial.coeff (Finsupp.equivFunOnFinite.symm c)
    ((∑ i : Fin (k + 1), MvPolynomial.X i) ^ m * h) ≠ 0) :
  let S : Finset (ZMod p) :=
    (Fintype.piFinset A).filter (fun f => h.eval f ≠ 0) |>.image (fun f => ∑
      i, f i)
  S.card ≥ m + 1 ∧ m < p := by
-- Define the restricted sumset S
set S : Finset (ZMod p) :=
  ((Fintype.piFinset A).filter (fun f => h.eval f ≠ 0)).image (fun f => ∑ i, f
    i) with hS_def

-- Step 1: Prove |S| ≥ m + 1 by contradiction

```

```

have hS_card : S.card ≥ m + 1 := by
  by_contra! H

have hS_size : S.card ≤ m := by omega
obtain ⟨E, hE_sub, hE_card⟩ : ∃ E : Multiset (ZMod p), S.val ⊆ E ∧ E.card =
  m := by
  refine ⟨S.val + Multiset.replicate (m - S.card) (0 : ZMod p),
    Multiset.subset_of_le (by simp), ?_⟩
  simp [hS_size]

-- Define the polynomial Q
set sumX : MvPolynomial (Fin (k + 1)) (ZMod p) := ∑ i, MvPolynomial.X i
  with hsumX_def
set Q : MvPolynomial (Fin (k + 1)) (ZMod p) :=
  h * (E.map (fun e => sumX - C e)).prod with hQ_def

-- Q vanishes on prod A_i
have hQ_zero : ∀ (x : Fin (k + 1) → ZMod p), (∀ i, x i ∈ A i) → eval x Q =
  0 := by
  intro x hx
  rw [hQ_def, eval_mul]
  by_cases hh : eval x h = 0
  • simp [hh]
  • have h_sum_in_S : (∑ i, x i) ∈ S := by
      simp [S, Fintype.mem_piFinset]
      refine ⟨x, ⟨hx, hh⟩, rfl⟩
  have h_sum_in_E : (∑ i, x i) ∈ E := hE_sub h_sum_in_S
  have : eval x ((E.map (fun e => sumX - C e)).prod) = 0 := by
    have mem : (sumX - C (∑ i, x i)) ∈ Multiset.map (fun e => sumX - C e)
      E :=
        Multiset.mem_map.mpr ⟨∑ i, x i, h_sum_in_E, rfl⟩
    have zero_eval : eval x (sumX - C (∑ i, x i)) = 0 := by
      simp [hsumX_def]
    have hprod_eq_zero : (MvPolynomial.eval x) (sumX - C (∑ i, x i)) = 0
      := by exact
        zero_eval
    have eval_factor_zero : eval x (sumX - C (∑ i, x i)) = 0 := by exact
      zero_eval
    have prod_zero :
      (MvPolynomial.eval x) (Multiset.map (fun e => sumX - C e) E).prod = 0
      := by
        have : (MvPolynomial.eval x) ((Multiset.map (fun e => sumX - C e) E
          ).prod) =
          (Multiset.map (fun e => (MvPolynomial.eval x) (sumX - C e)) E
            ).prod := by
          exact Eq.symm (Multiset.prod_hom' E (MvPolynomial.eval x) fun
            i ↦ sumX - C i)
        rw [this]
        subst hm

```

```

simp_all [S, sumX, Q]
obtain ⟨w, h_1⟩ := h_sum_in_S
obtain ⟨w_1, h_2⟩ := mem
obtain ⟨left, right⟩ := h_1
obtain ⟨left_1, right_1⟩ := h_2
obtain ⟨left, right_2⟩ := left
apply Exists.intro
• apply And.intro
  • apply h_sum_in_E
  • simp_all only [sub_self]
subst hm
simp_all [S, sumX, Q]
simp only [this, mul_zero]

have hQ_total_deg : Q.totalDegree =  $\sum i, c_i$  := by
rw [hQ_def, hsumX_def]
have h_prod_deg : ((E.map (fun e => sumX - C e)).prod).totalDegree = m :=
by
rw [hsumX_def]
have degree_of_each :  $\forall e : \text{ZMod } p, (\text{sumX} - C e).totalDegree = 1$  := by
intro e
rw [hsumX_def]
have :  $(\sum i : \text{Fin } (k + 1), X_i - C e) = (\sum i, X_i) + (-C e)$  := by rw
[sub_eq_add_neg]
rw [MvPolynomial.totalDegree]
apply le_antisymm
• refine Finset.sup_le fun d hd => ?_
simp [this] at hd
have :  $(d.\text{sum } fun x e \mapsto e) \leq 1$  := by
-- Step 1: Coefficient decomposition of sum  $X_i - C e$ 
have coeff_sub_eq :
coeff d  $(\sum i, X_i - C e) = \text{coeff } d (\sum i, X_i) + -\text{coeff } d (C e)$  :=
by
simp [MvPolynomial.coeff_sub]
exact sub_eq_add_neg (coeff d  $(\sum i, X_i)$ ) (if 0 = d then e else 0)
have coeff_C_eq :  $\text{coeff } d (C e) = \text{if } d = 0 \text{ then } e \text{ else } 0$  := by
simp [MvPolynomial.coeff_C]
subst hE_card
simp_all [S, sumX, Q]
split
next h_1 =>
  subst h_1
  simp_all only [↓reduceIte]
next h_1 =>
  simp_all only [↓reduceIte, neg_zero, add_zero,
    right_eq_ite_iff]
  intro a
  subst a

```

```

      simp_all only [not_true_eq_false]
rw [coeff_C_eq] at coeff_sub_eq
-- Step 2: d is in the support since its coefficient != 0
have mem_support : d ∈ (∑ i, X i - C e).support := by
  rw [MvPolynomial.mem_support_iff, coeff_sub_eq]
  subst hE_card
  simp_all [S, sumX, Q]
have support_subset :
(∑ i, X i - C e).support ⊆
  (Finset.biUnion Finset.univ fun i : Fin (k + 1) => {Finsupp.
    single i 1})
  ∪ {0} := by
intro x hx
rw [MvPolynomial.mem_support_iff] at hx
have coeff_eq : coeff x (∑ i, X i - C e) = coeff x (∑ i, X i) -
  coeff x (C e) := by
  simp [MvPolynomial.coeff_sub]
rw [coeff_eq] at hx
have coeff_sum_eq :
coeff x (∑ i, X i) = if ∃ i, x = Finsupp.single i 1 then 1 else
  0 := by
  simp [MvPolynomial.coeff_sum]
have h :
∑ x_1, coeff x (X x_1) = if ∃ i, x = Finsupp.single i 1 then
  1 else 0 := by
  by_cases h : ∃ i, x = Finsupp.single i 1
  • rcases h with ⟨i, hi⟩
    have :
    ∀ j, (if x = Finsupp.single j 1
    then (1 : ZMod p) else 0) = if i = j then 1 else 0
    :=
    by
      intro j
      rw [hi]
      by_cases h : i = j
      • subst h
        simp only [↓reduceIte]
      • simp [h]
        rw [@single_eq_single_iff]
        ring_nf
        simp_all
    aesop
  • push_neg at h
    simp [h]
    have : ∀ i, coeff x (X i) = 0 := by
      intro i
      simp [MvPolynomial.coeff_X']
      exact fun a ↦ h i (id (Eq.symm a))
    exact fun i => this i

```

```

      subst hm
      simp_all [S, sumX, Q]
    have coeff_C_eq : coeff x (C e) = if x = 0 then e else 0 := by
      simp [MvPolynomial.coeff_C]
      subst hm
      simp_all [S, sumX, Q]
    split
    next h_1 =>
      subst h_1
      simp_all only [↓reduceIte]
    next h_1 =>
      simp_all only [↓reduceIte, sub_zero, neg_zero, add_zero,
        right_eq_ite_iff]
      intro a
      subst a
      simp_all only [not_true_eq_false]
    by_cases h : ∃ i, x = Finsupp.single i 1
    • rcases h with ⟨i, hi⟩
      apply Finset.mem_union_left
      simp [hi]
      use i
    • rw [Finset.mem_union, Finset.mem_singleton]
      right
      have h1 : coeff x (∑ i, X i) = (0 : ZMod p) := by
        have : ¬∃ i, x = Finsupp.single i 1 := h
        sorry
      rw [h1] at hx
      rw [coeff_C_eq] at hx
      by_cases h2 : x = 0
      • exact h2
      • simp [h2] at hx
    have :
      d ∈ (Finset.biUnion Finset.univ fun i : Fin (k + 1) => {Finsupp.
        single i 1}) ∪ {0} :=
      support_subset mem_support
    simp at this
    subst hm
    simp_all only [S, sumX, Q]
    cases this with
    | inl h_1 =>
      subst h_1
      simp_all only [↓reduceIte, sum_zero_index, zero_le]
    | inr h_2 =>
      obtain ⟨w, h_1⟩ := h_2
      subst h_1
      simp_all only [single_eq_zero, one_ne_zero, ↓reduceIte,
        neg_zero, add_zero,
        sum_single_index, le_refl]
    exact this

```

```

simp
let b : (Fin (k + 1)) →0 ℕ := Finsupp.single (0 : Fin (k + 1)) 1
refine ⟨b, ?_, ?_⟩
• have coeff_eq : coeff (Finsupp.single (0 : Fin (k + 1)) 1) (∑ i, X
  i) = 1 := by
  simp [coeff_sum, coeff_X', Finsupp.single_eq_single_iff]
rw [show b = Finsupp.single (0 : Fin (k + 1)) 1 by rfl] at *
have h : coeff b (∑ i, X i) = 1 := by
  dsimp [b]
  exact coeff_eq
sorry
• simp only [sum_single_index, le_refl, b]
• sorry
have h_h_deg : h.totalDegree = (∑ i, c i) - m := by
  rw [hm]

  sorry
  sorry
--
have hQ_coeff : MvPolynomial.coeff (Finsupp.equivFunOnFinite.symm c) Q ≠ 0
  := by
  rw [hQ_def, coeff_mul]
  sorry

-- Define elimination polynomials g_i
set g : Fin (k + 1) → MvPolynomial (Fin (k + 1)) (ZMod p) :=
  elimination_polynomials A with hg_def

-- Construct Q_bar by reducing degrees
set Q_bar : MvPolynomial (Fin (k + 1)) (ZMod p) :=
  reduce_polynomial_degrees Q g c with hQ_bar_def

-- Now the key properties of Q_bar
have ⟨R, decomp⟩ :
  ∃ R, (E.map (fun e => sumX - C e)).prod = sumX^m + R :=
by
  refine ⟨(E.map (fun e => sumX - C e)).prod - sumX^m, ?_⟩
  simp

let target := Finsupp.equivFunOnFinite.symm c
let P := (E.map (fun e => sumX - C e)).prod

-- Q = h * P
have coeff_decomp :
  (Q.coeff target) =
    (h * sumX^m).coeff target + (h * R).coeff target :=
by sorry

-- Q_bar vanishes on prod A_i

```

```

have hQ_bar_zero :  $\forall (x : \text{Fin } (k + 1) \rightarrow \text{ZMod } p), (\forall i, x\ i \in A\ i) \rightarrow \text{eval } x$ 
  Q_bar = 0 := by
  intro x hx
  sorry

-- Q_bar has degree constraints
have hQ_bar_deg :  $\forall i, Q\_bar.\text{degreeOf } i \leq c\ i$  := by
  intro i
  sorry

have hQ_bar_zero_poly : Q_bar = 0 :=
  _root_.eq_zero_of_eval_zero_at_prod_finset Q_bar A (fun i => by
    have := hQ_bar_deg i
    grind) hQ_bar_zero

-- But the coefficient of the target monomial in Q_bar is nonzero
have hQ_bar_coeff : MvPolynomial.coeff (Finsupp.equivFunOnFinite.symm c)
  Q_bar  $\neq$  0 := by
  -- Note that the replacement process does not affect this coefficient
  sorry

-- Contradiction
rw [hQ_bar_zero_poly] at hQ_bar_coeff
simp at hQ_bar_coeff

-- Step 2: Prove  $m < p$  first (this is needed for the main argument)
have hmp :  $m < p$  := by
  by_contra! H -- H:  $m \geq p$ 
  -- If  $m \geq p$ , use the Frobenius endomorphism property in characteristic  $p$ 
  have frobenius_identity :  $((\sum i : \text{Fin } (k + 1), \text{MvPolynomial.X } i) ^ p : \text{MvPolynomial } (\text{Fin } (k + 1)) (\text{ZMod } p)) = \sum i, \text{MvPolynomial.X } i ^ p$  := by
    subst hm
    simp_all only [ne_eq, ge_iff_le, S]
    exact sum_pow_char p Finset.univ X

  -- This changes the structure of  $(\sum X_i)^m$  when  $m \geq p$ , leading to
  -- contradiction with h_coeff
  subst hm
  simp_all only [ne_eq, ge_iff_le, S]
  sorry -- Detailed argument needed here

exact ⟨hS_card, hmp⟩

```